Algoritmos Aproximados/Envasado.dfy/Envasado2Aproximado.dfy
@@ -1,9 +1,11 @@
 include "../../Especificaciones/Envasado/Envasado.dfy"
 include "EnvasadoKAproximado.dfy"
+include "Algoritmo2AproximadoAux.dfy"
 
 //We use the first fit strategy and check the elements in any order
 //At most only one bin is less than half full, thus we use most twice as many as in the optimal solution
 method binPacking2Aproximated(A: multiset<nat>, E: nat) returns (I: multiset<multiset<nat>>)
+requires forall a: nat | a in A :: a <= E
 //ensures isKAproximatedBinPacking(A, E, I, 2)
 {
     //Variable initialization
@@ -12,30 +14,98 @@ method binPacking2Aproximated(A: multiset<nat>, E: nat) returns (I: multiset<mul
     var capacity: seq<nat> := [];
     //iterateMultiset exists to let us iterate over all the elements in A, one by one
     var iterateMultiset: multiset<nat> := A;
+    ghost var analyzed: multiset<nat> := multiset{};
     I := multiset{};
     while iterateMultiset != multiset{}
     decreases iterateMultiset
     invariant |bins| == |capacity|
+    invariant iterateMultiset <= A 
+    invariant analyzed <= A 
+    invariant iterateMultiset + analyzed == A
+    invariant forall i: nat | 0 <= i < |bins| :: GSumNat(bins[i]) == capacity[i] && capacity[i] <= E
+    invariant isEnvasado(analyzed, E, I)
+    invariant I == multiset(bins)
+    //invariant allMoreThanHalfFullSeq(E, bins) || oneLessThanHalfFullSeq(E, bins)
     //at most  one bin is less than half full
     {
+        
         var currElement: nat := pickMultiset(iterateMultiset);
         var i := 0;
-        var fit: bool := false; 
+        var fit: bool := false;
+
+        assert Union(I) == analyzed;
+
         while !fit && i < |bins|
         invariant |bins| == |capacity|
+        invariant |bins| == |capacity|
+        invariant iterateMultiset <= A 
+        invariant analyzed <= A 
+        invariant iterateMultiset + analyzed == A
+        invariant forall i: nat | 0 <= i < |bins| :: GSumNat(bins[i]) == capacity[i] && capacity[i] <= E
+        invariant I == multiset(bins)
+        invariant !fit ==> Union(I) == analyzed
+        invariant fit ==> Union(I) == analyzed + multiset{currElement}
         {
+            assert capacity[i] == GSumNat(bins[i]);
             if capacity[i] + currElement < E {
+                
+                //assert Union(I) == analyzed + multiset{currElement};
+                //assume false;
+                //Proof for valid capacity
+                GSumIntElemIn(bins[i] + multiset{currElement}, currElement);
+                assert bins[i] + multiset{currElement} - multiset{currElement} == bins[i];
+                GSumPositiveIntNat(bins[i] + multiset{currElement});
+                GSumPositiveIntNat(bins[i]);
+                assert GSumNat(bins[i]) <= E;
+
+                ghost var I' := I - multiset{bins[i]};
+                ghost var bin := bins[i];
+                UnionOne(I, bin);
+                assert analyzed == bin + Union(I');
+                assert Union(I') == analyzed - bin;
+                ghost var bin' := bins[i] + multiset{currElement};
+                //requires B == A + multiset{C}
+                //ensures Union(B) == Union(A) + C
+                ghost var I'' := I' + multiset{bin'};
+                Union3(I', I'', bin');
+                calc{
+                    Union(I'');
+                    Union(I') + bin';
+                    analyzed - bin + bin';
+                    analyzed + multiset{currElement};
+                }
+                assert Union(I'') == analyzed + multiset{currElement};
+                assume false;
+                
+                //assert Union(I) == analyzed;
+                I := I - multiset{bins[i]};
                 bins := bins[i := (bins[i] + multiset{currElement})];
+                I := I + multiset{bins[i]};
+                assert I == I'';
+                var capacityBefore := capacity[i]; 
+                capacity := capacity[i := capacityBefore + currElement];
                 fit := true;
+
+                assert fit == true;
+            }
+            else{
+                assert fit == false;
             }
             i := i + 1;
-        }
+        } 
+        assume false;
+        //assume Union(multiset(bins)) == analyzed + multiset{currElement}; 
+        //assume false;
+        //assert forall x | x in multiset(bins) :: x <= analyzed + multiset{currElement} && GSumNat(x) <= E;
+        //assume false;
         //If no fit was found we must create another bin
         if !fit {
             bins := bins + [multiset{currElement}];
             capacity := capacity + [currElement];
+            I := I + multiset{multiset{currElement}};
         }
         iterateMultiset := iterateMultiset - multiset{currElement};
+        analyzed := analyzed + multiset{currElement};
     }
     I := multiset(bins);
 }
